steel/Zeta.Steel.ThreadSim.fsti
@@ -10,62 +10,43 @@ open Zeta.Steel.AddMRel
 module GV = Zeta.GenericVerifier
 module IV = Zeta.Intermediate.Verifier
 module T = Zeta.Steel.FormatsManual
+module LT = Zeta.Steel.LogEntry.Types
 
 val addm_simulation (tsm: s_thread_state) (i_tsm: i_thread_state) (se: s_log_entry) (ie: i_log_entry)
   : Lemma (requires (related_tsm tsm i_tsm /\
                      related_log_entry se ie /\
-                     T.AddM? se /\ not tsm.failed))
-          (ensures (let T.AddM p = se in
+                     LT.AddM? se /\ not tsm.failed))
+          (ensures (let LT.AddM s s' r = se in
                     let GV.AddM ir is is' = ie in
-                    let tsm_ = vaddm tsm p.s p.s' (Inl (p.k, p.v)) in
-                    let i_tsm_ = IV.addm ir is is' i_tsm in
-                    (not tsm_.failed) ==> related_tsm tsm_ i_tsm_))
-
-val addmapp_simulation (tsm: s_thread_state) (i_tsm: i_thread_state) (se: s_log_entry) (ie: i_log_entry)
-  : Lemma (requires (related_tsm tsm i_tsm /\
-                     related_log_entry se ie /\
-                     T.AddMApp? se /\ not tsm.failed))
-          (ensures (let T.AddMApp p = se in
-                    let GV.AddM ir is is' = ie in
-                    let tsm_ = vaddm tsm p.s p.s' (Inr p.rest) in
+                    let tsm_ = vaddm tsm s s' r in
                     let i_tsm_ = IV.addm ir is is' i_tsm in
                     (not tsm_.failed) ==> related_tsm tsm_ i_tsm_))
 
 val addb_simulation (tsm: s_thread_state) (i_tsm: i_thread_state) (se: s_log_entry) (ie: i_log_entry)
   : Lemma (requires (related_tsm tsm i_tsm /\
                      related_log_entry se ie /\
-                     T.AddB? se /\ not tsm.failed))
-          (ensures (let T.AddB p = se in
+                     LT.AddB? se /\ not tsm.failed))
+          (ensures (let LT.AddB s t tid r = se in
                     let GV.AddB i_r i_s i_t i_tid = ie in
-                    let tsm_ = vaddb tsm p.s p.t p.tid (Inl (p.k, p.v))  in
-                    let i_tsm_ = IV.addb i_r i_s i_t i_tid i_tsm in
-                    (not tsm_.failed) ==> related_tsm tsm_ i_tsm_))
-
-val addbapp_simulation (tsm: s_thread_state) (i_tsm: i_thread_state) (se: s_log_entry) (ie: i_log_entry)
-  : Lemma (requires (related_tsm tsm i_tsm /\
-                     related_log_entry se ie /\
-                     T.AddBApp? se /\ not tsm.failed))
-          (ensures (let T.AddBApp p = se in
-                    let GV.AddB i_r i_s i_t i_tid = ie in
-                    let tsm_ = vaddb tsm p.s p.t p.tid (Inr p.rest)  in
+                    let tsm_ = vaddb tsm s t tid r  in
                     let i_tsm_ = IV.addb i_r i_s i_t i_tid i_tsm in
                     (not tsm_.failed) ==> related_tsm tsm_ i_tsm_))
 
 val evictm_simulation (tsm: s_thread_state) (i_tsm: i_thread_state) (se: s_log_entry) (ie: i_log_entry)
   : Lemma (requires (related_tsm tsm i_tsm /\
                      related_log_entry se ie /\
-                     T.EvictM? se /\ not tsm.failed))
-          (ensures (let T.EvictM p = se in
+                     LT.EvictM? se /\ not tsm.failed))
+          (ensures (let LT.EvictM p = se in
                     let GV.EvictM i_s i_s' = ie in
-                    let tsm_ = vevictm tsm p.s p.s'  in
+                    let tsm_ = vevictm tsm p.s p.s_  in
                     let i_tsm_ = IV.evictm i_s i_s' i_tsm in
                     (not tsm_.failed) ==> related_tsm tsm_ i_tsm_))
 
 val evictb_simulation (tsm: s_thread_state) (i_tsm: i_thread_state) (se: s_log_entry) (ie: i_log_entry)
   : Lemma (requires (related_tsm tsm i_tsm /\
                      related_log_entry se ie /\
-                     T.EvictB? se /\ not tsm.failed))
-          (ensures (let T.EvictB p = se in
+                     LT.EvictB? se /\ not tsm.failed))
+          (ensures (let LT.EvictB p = se in
                     let GV.EvictB i_s i_t = ie in
                     let tsm_ = vevictb tsm p.s p.t in
                     let i_tsm_ = IV.evictb i_s i_t i_tsm in
@@ -74,17 +55,17 @@ val evictb_simulation (tsm: s_thread_state) (i_tsm: i_thread_state) (se: s_log_e
 val evictbm_simulation (tsm: s_thread_state) (i_tsm: i_thread_state) (se: s_log_entry) (ie: i_log_entry)
   : Lemma (requires (related_tsm tsm i_tsm /\
                      related_log_entry se ie /\
-                     T.EvictBM? se /\ not tsm.failed))
-          (ensures (let T.EvictBM p = se in
+                     LT.EvictBM? se /\ not tsm.failed))
+          (ensures (let LT.EvictBM p = se in
                     let GV.EvictBM i_s i_s' i_t = ie in
-                    let tsm_ = vevictbm tsm p.s p.s' p.t in
+                    let tsm_ = vevictbm tsm p.s p.s_ p.t in
                     let i_tsm_ = IV.evictbm i_s i_s' i_t i_tsm in
                     (not tsm_.failed) ==> related_tsm tsm_ i_tsm_))
 
 val nextepoch_simulation (tsm: s_thread_state) (i_tsm: i_thread_state) (se: s_log_entry) (ie: i_log_entry)
   : Lemma (requires (related_tsm tsm i_tsm /\
                      related_log_entry se ie /\
-                     T.NextEpoch? se /\ not tsm.failed))
+                     LT.NextEpoch? se /\ not tsm.failed))
           (ensures (let tsm_ = nextepoch tsm in
                     let i_tsm_ = IV.nextepoch i_tsm in
                     (not tsm_.failed) ==> related_tsm tsm_ i_tsm_))
@@ -92,7 +73,7 @@ val nextepoch_simulation (tsm: s_thread_state) (i_tsm: i_thread_state) (se: s_lo
 val verifyepoch_simulation (tsm: s_thread_state) (i_tsm: i_thread_state) (se: s_log_entry) (ie: i_log_entry)
   : Lemma (requires (related_tsm tsm i_tsm /\
                      related_log_entry se ie /\
-                     T.VerifyEpoch? se /\ not tsm.failed))
+                     LT.VerifyEpoch? se /\ not tsm.failed))
           (ensures (let tsm_ = verifyepoch tsm in
                     let i_tsm_ = IV.verifyepoch i_tsm in
                     (not tsm_.failed) ==> related_tsm tsm_ i_tsm_))
